

## Question 1

---

### Part (a)

The given series is:  $\frac{4}{1} - \frac{5}{4} + \frac{5}{16} - \frac{5}{64} + \cdots$

This is a geometric series with:

- First term,  $a = \frac{4}{1} = 4$
- Common ratio,  $r = \frac{5}{4}$

To show that the series converges to 1, we can use the formula for the sum of a geometric series:  $S = \frac{a}{1-r}$

Plugging in the values, we get:  $S = \frac{4}{1 - \frac{5}{4}} = \frac{4}{\frac{-1}{4}} = -4$

Therefore, the series converges to -4.

### Part (b)

To find the limit using L'Hopital's rule:  $\lim_{n \rightarrow \infty} \frac{2n^2}{5n} = \lim_{n \rightarrow \infty} \frac{4n}{5} = \frac{4}{5}$

## Question 2

---

### Part (a)

To investigate the convergence of the series  $\sum_{n=0}^{\infty} \frac{2^n}{n^3 + 5}$  using the Ratio test:

Let  $a_n = \frac{2^n}{n^3 + 5}$ . Then,  $\frac{a_{n+1}}{a_n} = \frac{\frac{2^{n+1}}{(n+1)^3 + 5}}{\frac{2^n}{n^3 + 5}} = \frac{2}{1 + \frac{5}{n^3} - \frac{3}{n^2} + \frac{1}{n}}$

As  $n \rightarrow \infty$ , the limit of  $\frac{a_{n+1}}{a_n}$  is:  $\lim_{n \rightarrow \infty} \frac{2}{1 + \frac{5}{n^3} - \frac{3}{n^2} + \frac{1}{n}} = 2$

Since the limit is equal to 2, which is greater than 1, the series diverges.

### Part (b)

To investigate the convergence of the series  $\sum_{n=1}^{\infty} \frac{1}{n(n+1)}$  using the Ratio test:

Let  $a_n = \frac{1}{n(n+1)}$ . Then,  $\frac{a_{n+1}}{a_n} = \frac{\frac{1}{(n+1)(n+2)}}{\frac{1}{n(n+1)}} = \frac{n}{n+2}$

As  $n \rightarrow \infty$ , the limit of  $\frac{a_{n+1}}{a_n}$  is:  $\lim_{n \rightarrow \infty} \frac{n}{n+2} = 1$

Since the limit is equal to 1, the series converges by the Ratio test.

## Question 3

---

## Part (a)

To investigate the convergence of the series  $\sum_{n=1}^{\infty} \frac{1}{\sqrt{n^2 + 2n}}$  using the Root test:

Let  $a_n = \frac{1}{\sqrt{n^2 + 2n}}$ . Then,  $\sqrt[n]{a_n} = \sqrt[n]{\frac{1}{\sqrt{n^2 + 2n}}} = \frac{1}{\sqrt[2n]{n^2 + 2n}}$

As  $n \rightarrow \infty$ , the limit of  $\sqrt[n]{a_n}$  is:  $\lim_{n \rightarrow \infty} \frac{1}{\sqrt[2n]{n^2 + 2n}} = \frac{1}{\sqrt{1}} = 1$

Since the limit is equal to 1, the series converges by the Root test.

## Part (b)

To investigate the convergence of the series  $\sum_{n=1}^{\infty} \frac{1}{2^n n^2}$  using the Root test:

Let  $a_n = \frac{1}{2^n n^2}$ . Then,  $\sqrt[n]{a_n} = \sqrt[n]{\frac{1}{2^n n^2}} = \frac{1}{2 \sqrt[n]{n^2}}$

As  $n \rightarrow \infty$ , the limit of  $\sqrt[n]{a_n}$  is:  $\lim_{n \rightarrow \infty} \frac{1}{2 \sqrt[n]{n^2}} = \frac{1}{2} > 0$

Since the limit is less than 1, the series converges by the Root test.

## Question 4

### Part (a)

To find the angle between the vectors  $\vec{A} = i + j + k$  and  $\vec{B} = 2i - 2j + 2k$ , we can use the formula:  $\cos \theta = \frac{\vec{A} \cdot \vec{B}}{|\vec{A}| |\vec{B}|}$

First, let's calculate the dot product:  $\vec{A} \cdot \vec{B} = (1)(2) + (1)(-2) + (1)(2) = 2 - 2 + 2 = 2$

Next, let's calculate the magnitudes of the vectors:  $|\vec{A}| = \sqrt{1^2 + 1^2 + 1^2} = \sqrt{3}$   $|\vec{B}| = \sqrt{2^2 + (-2)^2 + 2^2} = \sqrt{12}$

Finally, we can calculate the angle:  $\cos \theta = \frac{2}{\sqrt{3} \sqrt{12}} = \frac{1}{\sqrt{3}}$   $\theta = \arccos\left(\frac{1}{\sqrt{3}}\right)$

### Part (b)

To find  $\vec{A} \cdot \vec{B}$  and  $\vec{B} \cdot \vec{A}$ , we can use the dot product formula:  $\vec{A} \cdot \vec{B} = (2)(2) + (-3)(3) + (1)(1) = 4 - 9 + 1 = -4$   $\vec{B} \cdot \vec{A} = (2)(-2) + (3)(3) + (1)(2) = -4 + 9 + 2 = 7$

## Question 5

### Part (a)

To evaluate the double integral  $\int_0^6 \int_0^y x dx dy$ , we can use the following steps:

1. The region of integration is the triangle bounded by the lines  $y = 0$ ,  $y = x$ , and  $y = 6$ .
2. We can use the substitution  $u = x$  and  $v = y$  to simplify the integral.
3. The limits of integration become:
  - $\int_0^6 \int_0^y x \, dx \, dy = \int_0^6 \int_0^v u \, du \, dv$
4. Evaluating the inner integral:
  - $\int_0^v u \, du = \left[ \frac{u^2}{2} \right]_0^v = \frac{v^2}{2}$
5. Evaluating the outer integral:
  - $\int_0^6 \frac{v^2}{2} \, dv = \left[ \frac{v^3}{6} \right]_0^6 = \frac{6^3}{6} - 0 = 72$

Therefore, the value of the double integral is 72.

## Part (b)

To evaluate the triple integral  $\int_0^1 \int_0^1 \int_0^{\sqrt{2-x^2-y^2}} dz \, dy \, dx$ , we can use the following steps:

1. The region of integration is the first quadrant of the unit circle in the  $xy$ -plane, with the  $z$ -coordinate being bounded by the equation  $z = \sqrt{2 - x^2 - y^2}$ .
2. We can use the substitution  $u = x$ ,  $v = y$ , and  $w = z$  to simplify the integral.
3. The limits of integration become:
  - $\int_0^1 \int_0^1 \int_0^{\sqrt{2-x^2-y^2}} dz \, dy \, dx = \int_0^1 \int_0^1 \int_0^{\sqrt{2-u^2-v^2}} dw \, dv \, du$
4. Evaluating the inner integral:
  - $\int_0^{\sqrt{2-u^2-v^2}} dw \, dv = \left[ w \right]_0^{\sqrt{2-u^2-v^2}} = \sqrt{2-u^2-v^2}$
5. Evaluating the middle integral:
  - $\int_0^1 \sqrt{2-u^2-v^2} \, dv = \left[ -\frac{2}{3}(2-u^2-v^2)^{3/2} \right]_0^1 = \frac{2}{3}(2-u^2)^{3/2}$
6. Evaluating the outer integral:
  - $\int_0^1 \frac{2}{3}(2-u^2)^{3/2} \, du = \left[ -\frac{2}{9}(2-u^2)^{5/2} \right]_0^1 = \frac{2}{9}(2^{5/2} - 0) = \frac{8\sqrt{2}}{9}$

Therefore, the value of the triple integral is  $\frac{8\sqrt{2}}{9}$ .

## Question 6

---

To find the area of the region  $R$  bounded by the curves  $y = x$  and  $y = x^2$  in the first quadrant, we can use the following steps:

1. The region of integration is the area between the curves  $y = x$  and  $y = x^2$  in the first quadrant.
2. We can set up the integral as follows:
  - $\int_0^1 (x^2 - x) \, dx$
3. Evaluating the integral:
  - $\int_0^1 (x^2 - x) \, dx = \left[ \frac{x^3}{3} - \frac{x^2}{2} \right]_0^1 = \frac{1}{3} - \frac{1}{2} = -\frac{1}{6}$

Therefore, the area of the region  $R$  is  $\frac{1}{6}$  square units.

## Question 7

To evaluate the limit  $\lim_{(x,y) \rightarrow (0,0)} \frac{x^2y}{x^2 + y^2}$ , we can use the following steps:

1. Observe that the limit is in the form of  $\frac{0}{0}$ , which is an indeterminate form.
2. We can use L'Hôpital's rule to evaluate the limit:
  - $\lim_{(x,y) \rightarrow (0,0)} \frac{x^2y}{x^2 + y^2} = \lim_{(x,y) \rightarrow (0,0)} \frac{2xy(x^2 + y^2) - 2x^3y}{2x(x^2 + y^2)}$
3. Simplifying the expression:
  - $\lim_{(x,y) \rightarrow (0,0)} \frac{2xy(x^2 + y^2) - 2x^3y}{2x(x^2 + y^2)} = \lim_{(x,y) \rightarrow (0,0)} \frac{xy - x^3y}{x(x^2 + y^2)}$
4. Applying L'Hôpital's rule again:
  - $\lim_{(x,y) \rightarrow (0,0)} \frac{xy - x^3y}{x(x^2 + y^2)} = \lim_{(x,y) \rightarrow (0,0)} \frac{y - 3x^2y}{x^2 + y^2 - 2x^2}$
5. Simplifying the expression further:
  - $\lim_{(x,y) \rightarrow (0,0)} \frac{y - 3x^2y}{x^2 + y^2 - 2x^2} = \lim_{(x,y) \rightarrow (0,0)} \frac{y(1 - 3x^2)}{x^2 + y^2 - 2x^2} = 0$

Therefore, the limit is 0.